cleaning and renaming

Taskin/Right_Linear_Automata.thy
@@ -1,21 +1,28 @@
+subsection \<open>Relating Strongly Right-Linear Grammars and Automata\<close>
+
 theory Right_Linear_Automata
 imports
-  DFA_rlin2
+  NDA_rlin2
   "$AFP/Finite_Automata_HF/Finite_Automata_HF"
   HereditarilyFinite.Finitary
 begin
 
-subsection \<open>From Right-Linear Grammar to NFA\<close>
+subsection \<open>From Strongly Right-Linear Grammar to NFA\<close>
 
-definition nfa_rlin2 :: "('n,'t)prods \<Rightarrow> ('n::finitary) \<Rightarrow> 't nfa" where
-"nfa_rlin2 ps S =
-  \<lparr> states = hf_of  ` ({S} \<union> nts ps),
+definition nfa_rlin2 :: "('n,'t)Prods \<Rightarrow> ('n::finitary) \<Rightarrow> 't nfa" where
+"nfa_rlin2 P S =
+  \<lparr> states = hf_of  ` ({S} \<union> Nts P),
     init = {hf_of S},
-    final = hf_of ` {A \<in> nts ps. (A,[]) \<in> set ps},
-    nxt = \<lambda>q a. hf_of ` nxt_rlin2 (set ps) (inv hf_of q) a,
+    final = hf_of ` {A \<in> Nts P. (A,[]) \<in> P},
+    nxt = \<lambda>q a. hf_of ` nxt_rlin2 P (inv hf_of q) a,
     eps = Id \<rparr>"               
 
-interpretation NFA_rlin2: nfa "nfa_rlin2 ps S"
+context
+  fixes P :: "('n::finitary,'t)Prods"
+  assumes "finite P"
+begin
+
+interpretation NFA_rlin2: nfa "nfa_rlin2 P S"
 unfolding nfa_rlin2_def proof (standard, goal_cases)
   case 1
   then show ?case by(simp)
@@ -27,62 +34,59 @@ next
   then show ?case by(auto simp add: nxt_rlin2_nts)
 next
   case 4
-  then show ?case by (simp add: Nts_def finite_nts_syms split_def)
+  then show ?case using \<open>finite P\<close> by (simp add: Nts_def finite_nts_syms split_def)
 qed
 print_theorems
 
-lemma nfa_init_nfa_rlin2: "nfa.init (nfa_rlin2 ps S) = hf_of ` {S}"
+lemma nfa_init_nfa_rlin2: "nfa.init (nfa_rlin2 P S) = hf_of ` {S}"
 by (simp add: nfa_rlin2_def)
 
-lemma nfa_final_nfa_rlin2: "nfa.final (nfa_rlin2 ps S) = hf_of ` {A \<in> nts ps. (A,[]) \<in> set ps}"
+lemma nfa_final_nfa_rlin2: "nfa.final (nfa_rlin2 P S) = hf_of ` {A \<in> Nts P. (A,[]) \<in> P}"
 by (simp add: nfa_rlin2_def)
 
-lemma nfa_nxt_nfa_rlin2: "nfa.nxt (nfa_rlin2 ps S) (hf_of A) a = hf_of ` nxt_rlin2 (set ps) A a"
+lemma nfa_nxt_nfa_rlin2: "nfa.nxt (nfa_rlin2 P S) (hf_of A) a = hf_of ` nxt_rlin2 P A a"
 by (simp add: nfa_rlin2_def inj)
 
-lemma rtrancl_Id[simp]: "Id\<^sup>* = Id"
-by (metis rtrancl_empty rtrancl_idemp)
-
-lemma nfa_epsclo_nfa_rlin2: "M \<subseteq> {hf_of S} \<union> hf_of ` nts ps \<Longrightarrow> nfa.epsclo (nfa_rlin2 ps S) M = M"
+lemma nfa_epsclo_nfa_rlin2: "M \<subseteq> {hf_of S} \<union> hf_of ` Nts P \<Longrightarrow> nfa.epsclo (nfa_rlin2 P S) M = M"
 unfolding NFA_rlin2.epsclo_def unfolding nfa_rlin2_def by(auto)
 
-lemma nfa_nextl_nfa_rlin2: "M \<subseteq> {S} \<union> nts ps
-  \<Longrightarrow> nfa.nextl (nfa_rlin2 ps S) (hf_of ` M) xs = hf_of ` nxts_rlin2_set (set ps) M xs"
+lemma nfa_nextl_nfa_rlin2: "M \<subseteq> {S} \<union> Nts P
+  \<Longrightarrow> nfa.nextl (nfa_rlin2 P S) (hf_of ` M) xs = hf_of ` nxts_rlin2_set P M xs"
 proof(induction xs arbitrary: M)
   case Nil
   then show ?case
     by (simp add: nxts_rlin2_set_def)(fastforce intro!: nfa_epsclo_nfa_rlin2)
 next
   case (Cons a xs)
-  let ?epsclo = "nfa.epsclo (nfa_rlin2 ps S)"
-  let ?nxt = "nfa.nxt (nfa_rlin2 ps S)"
-  let ?nxts = "nfa.nextl (nfa_rlin2 ps S)"
+  let ?epsclo = "nfa.epsclo (nfa_rlin2 P S)"
+  let ?nxt = "nfa.nxt (nfa_rlin2 P S)"
+  let ?nxts = "nfa.nextl (nfa_rlin2 P S)"
   have "?nxts (hf_of ` M) (a # xs) = ?nxts (\<Union>x\<in>?epsclo (hf_of ` M). ?nxt x a) xs"
     by simp
   also have "\<dots> = ?nxts (\<Union>x\<in>hf_of ` M. ?nxt x a) xs"
     using Cons.prems by(subst nfa_epsclo_nfa_rlin2) auto
   also have "\<dots> = ?nxts (\<Union>m\<in>M. ?nxt (hf_of m) a) xs" by simp
-  also have "\<dots> = ?nxts (\<Union>m\<in>M. hf_of ` nxt_rlin2 (set ps) m a) xs"
+  also have "\<dots> = ?nxts (\<Union>m\<in>M. hf_of ` nxt_rlin2 P m a) xs"
     by (simp add: nfa_nxt_nfa_rlin2)
-  also have "\<dots> = ?nxts (hf_of ` (\<Union>m\<in>M. nxt_rlin2 (set ps) m a)) xs"
+  also have "\<dots> = ?nxts (hf_of ` (\<Union>m\<in>M. nxt_rlin2 P m a)) xs"
     by (metis image_UN)
-  also have "\<dots> = hf_of ` nxts_rlin2_set (set ps) (\<Union>m\<in>M. nxt_rlin2 (set ps) m a) xs"
+  also have "\<dots> = hf_of ` nxts_rlin2_set P (\<Union>m\<in>M. nxt_rlin2 P m a) xs"
     using Cons.prems by(subst Cons.IH)(auto simp add: nxt_rlin2_nts)
-  also have "\<dots> = hf_of ` nxts_rlin2_set (set ps) M (a # xs)"
+  also have "\<dots> = hf_of ` nxts_rlin2_set P M (a # xs)"
     by (simp add: nxt_rlin2_set_def nxts_rlin2_set_def)
   finally show ?case .
 qed
 
-lemma lang_pres_nfa_rlin2: assumes "rlin2 (set ps)"
-shows "nfa.language (nfa_rlin2 ps S) = CFG.lang ps S"
+lemma lang_pres_nfa_rlin2: assumes "rlin2 P"
+shows "nfa.language (nfa_rlin2 P S) = CFG.Lang P S"
 proof -
-  have 1: "\<And>A xs. \<lbrakk> A \<in> nxts_rlin2_set (set ps) {S} xs; A \<in> nts ps; (A, []) \<in> set ps\<rbrakk> \<Longrightarrow>
-    set ps \<turnstile> [Nt S] \<Rightarrow>* map Tm xs"
+  have 1: "\<And>A xs. \<lbrakk> A \<in> nxts_rlin2_set P {S} xs; A \<in> Nts P; (A, []) \<in> P\<rbrakk> \<Longrightarrow>
+    P \<turnstile> [Nt S] \<Rightarrow>* map Tm xs"
     using nxts_to_mult_derive by (metis (no_types, opaque_lifting) append.right_neutral derive.intros
       r_into_rtranclp rtranclp_trans singletonD)
-  have "\<And>A B. Nt B \<notin> syms ps \<Longrightarrow> (A, []) \<in> set ps \<Longrightarrow> A \<noteq> B" by(auto simp: Syms_def)
-  hence 2: "\<And>xs. rlin2 (set ps) \<Longrightarrow> set ps \<turnstile> [Nt S] \<Rightarrow>* map Tm xs \<Longrightarrow>
-          nxts_rlin2_set (set ps) {S} xs \<inter> {A \<in> nts ps. (A, []) \<in> set ps}  \<noteq> {}"
+  have "\<And>A B. Nt B \<notin> Syms P \<Longrightarrow> (A, []) \<in> P \<Longrightarrow> A \<noteq> B" by(auto simp: Syms_def)
+  hence 2: "\<And>xs. rlin2 P \<Longrightarrow> P \<turnstile> [Nt S] \<Rightarrow>* map Tm xs \<Longrightarrow>
+          nxts_rlin2_set P {S} xs \<inter> {A \<in> Nts P. (A, []) \<in> P} \<noteq> {}"
    using in_Nts_iff_in_Syms mult_derive_to_nxts rlin2_tms_eps
    by (metis (no_types, lifting) Int_Collect empty_iff singletonI)
   show ?thesis
@@ -91,11 +95,18 @@ proof -
     using 2[OF assms] by (auto simp: 1)
 qed
 
-subsection \<open>From DFA to Right-Linear Grammar\<close>
+lemma regular_if_rlin2: assumes "rlin2 P"
+  shows "regular (CFG.Lang P S)"
+using lang_pres_nfa_rlin2[OF assms] NFA_rlin2.imp_regular[of S]
+by metis
+
+end
+
+
+subsection \<open>From DFA to Strongly Right-Linear Grammar\<close>
 
 context dfa
 begin
-(* at the end: \<open>hf \<rightarrow> 'n::finitary\<close>, add \<open>hf_of \<dots>\<close> where needed *)
 
 text
 \<open>We define \<open>Prods_dfa\<close> that collects the production set from the deterministic finite automata \<open>M\<close>\<close>
@@ -175,9 +186,13 @@ next
   qed
 qed
 
-lemma "dfa.language M = Lang Prods_dfa (dfa.init M)"
+lemma dfa_language_eq_Lang: "dfa.language M = Lang Prods_dfa (dfa.init M)"
 unfolding language_def Lang_def by (simp add: Prods_dfa_iff_dfa)
 
 end
+
+lemma rlin2_if_regular: assumes "regular L"
+  shows "\<exists>P S::hf. rlin2 P \<and> L = CFG.Lang P S"
+by (metis assms dfa.dfa_language_eq_Lang dfa.rlin2_prods_dfa regular_def)
 
 end
